
> [!question]- #schols ![[Pasted image 20240703144541.png]]
 $\begin{vmatrix} 2 - \lambda & 1 & 1 \\ 1 & 2 - \lambda & 1 \\ 1 & 1 & 2 - \lambda \end{vmatrix} = 0$ 
 $A = (2 - \lambda)((2-\lambda)^2 - 1)$
 $A = (2 - \lambda)(4 - 4 \lambda + \lambda^2 - 1)$
 $A = (2 - \lambda)(\lambda^2 - 4 \lambda + 3)$
 $A = 2\lambda^2 - 8 \lambda + 6 - \lambda^3 + 4 \lambda^2 - 3 \lambda$
 $B = -(2 - \lambda - 1) = -1 + \lambda$ 
 $C = (1 - (2 - \lambda)) = -1 + \lambda$ 
 $A + B + C = 0$
 $-\lambda^3 + 6 \lambda^2 - 11 \lambda + 6 - 2 + 2 \lambda = 0$
 $-\lambda^3 + 6\lambda^2 - 9 \lambda + 4 = 0$
 $\lambda^3 - 6\lambda^2 + 9\lambda - 4 = 0$
 $\lambda = 1$
 $(\lambda - 1)(a\lambda^2 + b\lambda + c) = \lambda^3 - 6\lambda^2 + 9\lambda - 4$
 $a\lambda^3 + b\lambda^2 + c \lambda - a \lambda^2 - b \lambda - c$
 $a = 1$
 $c = 4$
 $b - 1 = -6$
 $b = -5$
 $\lambda^2 - 5 \lambda + 4 = 0$
 $\lambda = 1, 4, 1$ 
 $\begin{bmatrix} 1 & 1 & 1 & 0 \\ 1 & 1 & 1 & 0 \\ 1 & 1 & 1 & 0 \end{bmatrix}$
 $x_1 + x_2 + x_3 = 0$ 
 $v = \begin{bmatrix} -s - t \\ s \\ t \end{bmatrix}$ 
 $\begin{bmatrix} -2 & 1 & 1 & 0 \\ 1 & -2 & 1 & 0 \\ 1 & 1 & -2 & 0 \end{bmatrix}$
 $\begin{bmatrix} 1 & 1 & -2 & 0 \\ -2 & 1 & 1 & 0 \\ 1 & -2 & 1 & 0 \end{bmatrix}$
 $\begin{bmatrix} 1 & 1 & -2 & 0 \\ 0 & 3 & -3 & 0 \\ 0 & -3 & 3 & 0 \end{bmatrix}$
 $\begin{bmatrix} 1 & 1 & -2 & 0 \\ 0 & 1 & -1 & 0 \\ 0 & -1 & 1 & 0 \end{bmatrix}$
 $\begin{bmatrix} 1 & 0 & -1 & 0 \\ 0 & 1 & -1 & 0 \\ 0 & 0 & 0  & 0 \end{bmatrix}$ 
 $x_1 = x_3$
 $x_2 = x_3$
 $v = t \begin{bmatrix} 1 \\ 1 \\ 1 \end{bmatrix}$ 
 $P = \begin{bmatrix} -2 & 1 & -4 \\ 1 & 1 & 2 \\ 1 & 1 & 2 \end{bmatrix}$ 
