
![[Pasted image 20240702155832.png]]

![[Pasted image 20240905142718.png]]

> [!question]- #schols  ![[Pasted image 20240703144956.png]]
> $-2x + 4y - 8z = -18$
> $2x - 3y + z = 4$
> $y - 7z = -16$
> $y = \{0, 1\}$
> $0 - 7z = -16$
> $z = \dfrac{16}{7}$
> $1 - 7z = -16$
> $z = \dfrac{17}{7}$
> $x - 0 + 4(\dfrac{16}{7}) = 9$
> $x = -\dfrac{1}{7}$
> $x - 2(1) + 4(\dfrac{17}{7}) = 9$
> $x = \dfrac{9}{7}$
> $p_1 = (-\dfrac{1}{7}, 0, \dfrac{16}{7}), p_2 = (\dfrac{9}{7}, 1, \dfrac{17}{7})$
> $u = p_2 - p_1 = (\dfrac{10}{7}, 1, \dfrac{1}{7})$
> $X = P - ut$
> $x = \dfrac{9}{7} + \dfrac{10}{7}t$
> $y = 1 + t$
> $z = \dfrac{17}{7} + \dfrac{1}{7} t$

#NeedsFactCheckingByTrueAmericanPatriots 
> [!question] #schols [2024] ![[Pasted image 20241027191019.png]]
(i)
Make equation parametric to get vector, find perp vector, use implicit line eq formula
$2x - 6 = y - 3 = -2z$
$2x - 3 = y$
$z = 3 - x$
$v = (x, 2x - 3, 3 - x) = (0, -3, 3)$
$v \cdot u = 0$
$0u_x -3 u_y + 3u_z = 0$
 $u_y = u_z$ 
$u = (1, 1, 1)$
$\dfrac{x - 1}{1} = \dfrac{y + 2}{1} = \dfrac{z - 0}{1}$
 $x - 1 = y + 2 = z$ 
(ii)
 $-3x + 3y + 9z = 6$
 $10z = 15$
 $z = 3/2$ 
 $v = (0, 0, 3/2)$
 $v \cdot u = 0$
 $0u_x + 0u_y + 3/2 u_z = 0$
 $u_z = 0$
 $u = (1, 1, 0)$ 
 $X = P + ut$ 
 $x = 1 + t$
 $y = -2 + t$
 $z = 0$ 
 